warblreequiv/TMatcherEquivLemmas.v
@@ -1,0 +1,74 @@
+From Linden Require Import TMatcherEquivDef TreeMSInterp Tree.
+From Warblre Require Import Result Notation Base Errors.
+Import Notation.
+Import Result.Notations.
+
+Local Open Scope result_flow.
+
+Lemma equiv_choice:
+  forall (ms: MatchState) (gl: open_groups) resopt1 topt1 resopt2 topt2,
+    equiv_results topt1 ms gl resopt1 -> equiv_results topt2 ms gl resopt2 ->
+    equiv_results (
+        let! z =<< topt1 in
+        let! z' =<< topt2 in
+        Success (Choice z z')
+      ) ms gl (
+        let! z =<< resopt1 in
+        if (z !=? None)%wt then
+          Success z
+        else
+          resopt2
+      ).
+Proof.
+  intros ms gl resopt1 topt1 resopt2 topt2 Hequiv1 Hequiv2.
+  inversion Hequiv1 as [ t1 ms' gl' res1 Hequiv1' Heqt1 Heqms' Heqgl' Heqres1 |
+                       | ].
+  2,3: constructor.
+  subst ms' gl'.
+  inversion Hequiv2 as [ t2 ms' gl' res2 Hequiv2' Heqt2 Heqms' Heqgl' Heqres2 |
+                       | ]; simpl.
+  - replace (if (res1 !=? None)%wt then _ else _)
+      with (Success (F := MatchError) (if (res1 !=? None)%wt then res1 else res2
+           )) by now destruct res1.
+    constructor.
+    simpl.
+    rewrite <- Hequiv1'.
+    rewrite <- Hequiv2'.
+    now destruct res1.
+  - constructor.
+  - (* Something is happening here; may be simplified later *)
+    destruct res1; simpl. 2: constructor.
+    destruct topt2.
+    + simpl. constructor. simpl. rewrite <- Hequiv1'. reflexivity.
+    + constructor.
+Qed.
+
+Lemma func_monad_swap {F} `{Result.AssertionError F}:
+  forall topt1 topt2 (f1 f2: tree -> tree),
+    (let! t1 =<< topt1 in
+     let! t2 =<< topt2 in
+     Success (F := F) (Choice (f1 t1) (f2 t2))
+    ) = (
+          let! t1 =<<
+               let! t1 =<< topt1 in
+               Success (F := F) (f1 t1)
+          in
+          let! t2 =<<
+               let! t2 =<< topt2 in
+               Success (F := F) (f2 t2)
+          in
+          Success (F := F) (Choice t1 t2)
+        ).
+Proof.
+  intros topt1 topt2 f1 f2.
+  destruct topt1; destruct topt2; simpl; reflexivity.
+Qed.
+
+Lemma monad_id {T F} `{Result.AssertionError F}:
+  forall res: Result T F,
+    (let! x =<< res in Success x) = res.
+Proof.
+  intro res.
+  now destruct res.
+Qed.
+
